lean/LoVe/LoVe02_ProgramsAndTheorems_HomeworkSheet.lean
@@ -21,13 +21,18 @@ namespace LoVe
 end of a list. Your function should be defined by recursion and not using `++`
 (`List.append`). -/
 
-def snoc {α : Type} : List α → α → List α :=
-  sorry
+def snoc {α : Type} : List α → α → List α
+  | [], y => [y]
+  | x::xs, y => x :: snoc xs y
 
 /- 1.2 (1 point). Convince yourself that your definition of `snoc` works by
 testing it on a few examples. -/
 
 #eval snoc [1] 2
+#eval snoc [1,2,3,4] 5
+#eval snoc [1,2,3,4,5,6] 10
+#eval snoc [] 2
+
 -- invoke `#eval` or `#reduce` here
 
 
@@ -36,8 +41,9 @@ testing it on a few examples. -/
 2.1 (3 points). Define a `sum` function that computes the sum of all the numbers
 in a list. -/
 
-def sum : List ℕ → ℕ :=
-  sorry
+def sum : List ℕ → ℕ
+  | [] => 0
+  | x::xs => x + sum xs
 
 #eval sum [1, 12, 3]   -- expected: 16
 
@@ -51,5 +57,11 @@ def sum : List ℕ → ℕ :=
 Try to give meaningful names to your theorems. Use `sorry` as the proof. -/
 
 -- enter your theorem statements here
+
+theorem sum1 (ms : List ℕ) (n : ℕ) : sum (snoc ms n) = n + sum ms := by sorry
+
+theorem sum2 (ms ns : List ℕ) : sum (ms ++ ns) = sum ms + sum ns := by sorry
+
+theorem sum3 (ns : List ℕ) : sum (reverse ns) = sum ns := by sorry
 
 end LoVe
